Refactor + Simulation Soundness

theories/Commons/Language.v
@@ -1,48 +1,83 @@
 From stdpp Require Import prelude.
 
-Section language_mixin.
-  Context {state value : Type}.
+From RSL Require Import Commons.Utils.
 
-  Context (step : state -> state -> Prop).
+(* Set Mangle Names. *)
 
-  Context (can_progress : state -> Prop).
+Section lang_mixin.
+  Context {prog state value : Type}.
+
+  Context (step_rel : prog -> state -> state -> Prop).
+  Context (can_progress : prog -> state -> Prop).
+
   Context (is_final : state -> option value).
 
-  Record LanguageMixin := {
-      mixin_final_no_progress : ∀ s v, is_final s = Some v -> can_progress s -> False;
-      mixin_can_progress_must_step : ∀ s, can_progress s -> ∃ t, step s t;
-    }.
-End language_mixin.
+  Record LangMixin := {
+      mixin_final_no_progress:
+      ∀ p s v, is_final s = Some v -> ~can_progress p s;
+      mixin_final_no_step:
+      ∀ p s t v, is_final s = Some v -> ~step_rel p s t;
+      mixin_can_progress_must_step:
+      ∀ p s, can_progress p s -> ∃ t, step_rel p s t;
+     }.
+End lang_mixin.
 
-Structure language :=
-  Language {
+Structure lang :=
+  Lang
+    {
+      prog : Type;
       state : Type;
       value : Type;
 
-      step : state -> state -> Prop;
+      step_rel : prog -> state -> state -> Prop;
 
-      can_progress : state -> Prop;
+      can_progress : prog -> state -> Prop;
       is_final : state -> option value;
 
-      language_mixin : LanguageMixin step can_progress is_final;
+      lang_mixin : LangMixin step_rel can_progress is_final;
     }.
 
-Arguments step {_} _ _.
-Arguments can_progress {_} _.
-Arguments is_final {_}.
+Arguments step_rel {_} _ _ _.
+Arguments can_progress {_} _ _.
+Arguments is_final {_} _.
 
-Section Language.
-  Context {Λ: language}.
+Notation "P ⊨ s '->>' t" := (step_rel P s t) (at level 60, right associativity).
+Notation "P ⊨ s '-{' n '}>' t" := (nsteps (step_rel P) n s t) (at level 60, right associativity).
+Notation "P ⊨ s '->>*' t" := (rtc (step_rel P) s t) (at level 60, right associativity).
+Notation "P ⊨ s '->>+' t" := (psteps (step_rel P) s t) (at level 60, right associativity).
 
-  Definition stuck (s : state Λ) : Prop :=
-    is_final s = None ∧ ~ can_progress s.
+Section Stuck.
+  Context {Λ: lang} (P: prog Λ).
+
+  Definition stuck (s: state Λ) : Prop :=
+    is_final s = None ∧ ~ can_progress P s.
 
   Lemma final_not_stuck : ∀ s v,
     is_final s = Some v -> ~ stuck s.
   Proof. intros ? ? H [? ?]. inv H. Qed.
 
   Lemma progress_not_stuck : ∀ s,
-    can_progress s -> ~ stuck s.
+    can_progress P s -> ~ stuck s.
   Proof. intros ? ? []. tauto. Qed.
+End Stuck.
 
-End Language.
+Tactic Notation "mixin" :=
+  match goal with
+  | [ Hf: is_final ?s = Some _, Hp: can_progress _ ?s |- _ ] =>
+      exfalso;
+      eapply mixin_final_no_progress;
+      [apply lang_mixin | apply Hf | apply Hp]
+  | [ Hf: is_final ?s = Some _, Hs: _ ⊨ ?s ->> _ |- _ ] =>
+      exfalso;
+      eapply mixin_final_no_step;
+      [apply lang_mixin | apply Hf | apply Hs]
+  | [ Hf: is_final ?s = Some _, Hs: stuck _ ?s |- _ ] =>
+      let Hnfin := fresh "Hnfin" in
+      destruct Hs as [Hnfin _];
+      rewrite Hnfin in Hf;
+      discriminate Hf
+  | [ Hs: stuck ?P ?s, Hp: can_progress ?P ?s |- _ ] =>
+      let Hnp := fresh "Hnp" in
+      destruct Hs as [_ Hnp];
+      exfalso; apply (Hnp Hp)
+  end.
