theories/Commons/Logic.v
@@ -1,0 +1,176 @@
+From stdpp Require Import base.
+
+From RSL Require Import RTL.
+
+(* Set Mangle Names. *)
+
+Definition postcondition : Type := (val * memory) -> Prop.
+Definition precondition : Type := list val -> memory -> Prop.
+
+Definition logic : Type := regmap -> memory -> nat -> Prop.
+
+Declare Scope logic_scope.
+Delimit Scope logic_scope with logic.
+Bind Scope logic_scope with logic.
+
+Definition logic_and (P Q: logic) : logic :=
+  fun ρ m n => P ρ m n ∧ Q ρ m n.
+Definition logic_or (P Q: logic) : logic :=
+  fun ρ m n => P ρ m n ∨ Q ρ m n.
+Definition logic_impl (P Q: logic) : logic :=
+  fun ρ m n => P ρ m n -> Q ρ m n.
+Definition logic_not (P: logic) : logic :=
+  fun ρ m n => ~ P ρ m n.
+Definition logic_exists {X: Type} (f: X -> logic) : logic :=
+  fun ρ m n => ∃ x, f x ρ m n.
+Definition logic_forall {X: Type} (f: X -> logic) : logic :=
+  fun ρ m n => ∀ x, f x ρ m n.
+
+Definition logic_empty_entails (P: logic) : Prop :=
+  ∀ ρ m n, P ρ m n.
+Definition logic_pure (P: Prop) : logic :=
+  fun _ _ _ => P.
+Definition logic_memory_pure (P: memory -> Prop) : logic :=
+  fun _ m _ => P m.
+Definition logic_later (P: logic) : logic :=
+  fun ρ m n =>
+    match n with
+    | O => True
+    | S n => P ρ m n
+    end.
+
+Definition logic_always (P: logic) : logic :=
+  fun ρ m _ => ∀ n, P ρ m n.
+Definition logic_memory_entails (P: logic) : logic :=
+  fun ρ _ n => ∀ m, P ρ m n.
+Definition logic_register_entails (P: logic) : logic :=
+  fun _ m n => ∀ ρ, P ρ m n.
+
+Notation "P ∧ Q" :=
+  (logic_and P Q) : logic_scope.
+Notation "P ∨ Q" :=
+  (logic_or P Q)  : logic_scope.
+Notation "P -> Q" :=
+  (logic_impl P Q) : logic_scope.
+Notation "~ P" :=
+  (logic_not P) : logic_scope.
+Notation "'∃' x .. y , p" :=
+  (logic_exists (fun x => .. (logic_exists (fun y => p)) ..)) : logic_scope.
+Notation "'∀' x .. y , p" :=
+  (logic_forall (fun x => .. (logic_forall (fun y => p)) ..)) : logic_scope.
+
+Notation "⊢ P" :=
+  (logic_empty_entails P%logic)
+    (at level 99, right associativity).
+Notation "⌜ P ⌝" :=
+  (logic_pure P)
+    (at level 0, format "⌜ P ⌝") : logic_scope.
+Notation "⌜ P ⌝ₘ" :=
+  (logic_memory_pure P)
+    (at level 0, format "⌜ P ⌝ₘ") : logic_scope.
+Notation "▷ P" :=
+  (logic_later P)
+    (at level 20, right associativity, format "▷ P") : logic_scope.
+Notation "□ P" :=
+  (logic_always P)
+    (at level 20, right associativity, format "□ P") : logic_scope.
+Notation "'⊢ₘ' P" :=
+  (logic_memory_entails P)
+    (at level 99, right associativity) : logic_scope.
+Notation "'⊢ᵨ' P" :=
+  (logic_register_entails P)
+    (at level 99, right associativity) : logic_scope.
+
+Notation "'⟨' P '⟩'" := P%logic.
+
+(* Definition logic_entails `{Logic L} (P Q : L) : Prop := *)
+(*   logic_empty_entails (logic_impl P Q). *)
+(* Notation "P ⊢ Q" := *)
+(*   (logic_entails P%logic Q%logic) *)
+(*     (at level 99, right associativity). *)
+
+Definition logic_set_mem (addr: val) (v: val) (P: logic) : logic :=
+  fun ρ m n => ∃ m', set_at addr v m = Some m' ∧ P ρ m' n.
+
+Definition logic_assert_mem (addr: val) (v: val) : logic :=
+  fun _ m _ => get_at addr m = Some v.
+
+Definition logic_set_reg (r : reg) (v : val) (P : logic) : logic :=
+  fun ρ m n => P (set_reg r v ρ) m n.
+
+Notation "'⟦' addr '<-' v '⟧' P" :=
+  (logic_set_mem addr v P)
+    (at level 20, P at level 20, right associativity,
+       format "⟦ addr <- v ⟧  P").
+
+Notation "l '↦' v" :=
+  (logic_assert_mem l v)
+    (at level 70, no associativity, format "l ↦ v") : logic_scope.
+
+Notation "'⟦' dst '<-ᵣ' v '⟧' P" :=
+  (logic_set_reg dst v P)
+    (at level 20, P at level 20, right associativity,
+       format "⟦ dst <-ᵣ v ⟧  P") : logic_scope.
+
+Class LogicAssertReg (R V : Type) := logic_assert_reg : R -> V -> logic.
+
+Notation "r '↦ᵣ' v" :=
+  (logic_assert_reg r v)
+    (at level 70, no associativity, format "r ↦ᵣ v").
+
+Instance assert_reg_single : LogicAssertReg reg val :=
+  fun (r: reg) (v: val) ρ _ _ => get_reg r ρ = v.
+
+Instance assert_reg_list : LogicAssertReg (list reg) (list val) :=
+  fun (r: list reg) (v: list val) ρ _ _ => get_regs r ρ = v.
+
+Create HintDb custom_anyProp discriminated.
+
+Hint Unfold
+  (* lift_oProp *)
+  logic_and
+  logic_or
+  logic_impl
+  logic_not
+  logic_exists
+  logic_forall
+  (* logic_entails *)
+  logic_empty_entails
+  logic_pure
+  logic_memory_pure
+  logic_later
+  logic_always
+  logic_memory_entails
+  logic_register_entails
+
+  logic_set_mem
+  logic_assert_mem
+
+  logic_set_reg
+  logic_assert_reg
+
+  logic_assert_reg
+  assert_reg_single
+  assert_reg_list
+
+: custom_anyProp.
+
+Ltac unfold_Prop :=
+  autounfold with custom_anyProp in *;
+  cbv beta in *;
+  simpl in *.
+
+Lemma löb_weak P :
+  (⊢ ▷ P -> P) -> ⊢ P.
+Proof.
+  intros H ρ m n.
+  induction n as [|n IH]; now apply H.
+Qed.
+
+Lemma löb P :
+  (⊢ ▷ (⊢ᵨ ⊢ₘ P) -> P) -> ⊢ P.
+Proof.
+  intros H ρ m n.
+  revert ρ m.
+  induction n as [|n IH]; intros ρ m; now apply H.
+Qed.
