theories/Commons/Utils.v
@@ -1,0 +1,68 @@
+From stdpp Require Import prelude.
+
+Lemma nsteps_inv_l {A : Type} {R : relation A} :
+  ∀ n x z, nsteps R (S n) x z → ∃ y : A, R x y ∧ nsteps R n y z.
+Proof. intros n x z H; inv H; eexists; eauto. Qed.
+
+Variant psteps {A: Type} (R: relation A) : relation A :=
+| pstep_intro x y z : R x y -> rtc R y z -> psteps R x z.
+
+Lemma pstep_inv_l {A: Type} {R : relation A} :
+  ∀ x z, psteps R x z <-> ∃ y : A, R x y ∧ rtc R y z.
+Proof.
+  intros x z. split; intros H.
+  - inv H; eexists; now eauto.
+  - destruct H as (y & Hstep & Hrtc). econstructor; now eauto.
+Qed.
+
+Lemma pstep_inv_r {A: Type} {R : relation A} :
+  ∀ x z, psteps R x z <-> ∃ y : A, rtc R x y ∧ R y z.
+Proof.
+  intros x z; split; intros H.
+  - inv H as [? ? ? Hs Hrtc].
+    induction Hrtc as [y | x' y z Hstep Hrtc IH ] in x, y, z, Hrtc, Hs |- *.
+    + exists x; split; eauto; constructor.
+    + apply IH in Hstep. destruct Hstep as (y' & ? & ?).
+      eexists; split; eauto; econstructor; now eauto.
+  - destruct H as (y & Hrtc & Hstep).
+    inv Hrtc.
+    + repeat econstructor; assumption.
+    + econstructor; eauto. eapply rtc_r; eassumption.
+Qed.
+
+Lemma pstep_nsteps {A: Type} {R : relation A} :
+  ∀ x y, psteps R x y <-> ∃ n, nsteps R n x y ∧ n > 0.
+Proof.
+  intros x y; split; intros H.
+  - inv H as [a b c Hstep Hrtc]. apply rtc_nsteps_1 in Hrtc.
+    destruct Hrtc as [n Hnsteps]. eexists (S n); split; try lia.
+    econstructor; eassumption.
+  - destruct H as [[] [Hstep Hlt]]; try lia.
+    inv Hstep as [ | ? ? ? ? Hr Hnsteps ]. apply rtc_nsteps_2 in Hnsteps.
+    econstructor; eassumption.
+Qed.
+
+Definition EM := ∀ P, P ∨ ~P.
+
+Section ClassicalFacts.
+  Hypothesis EM : EM.
+
+  Lemma DNE P : ~~P -> P.
+  Proof. pose proof (EM P). tauto. Qed.
+
+  Lemma not_ex_all_not {T: Type} (P: T -> Prop) :
+    ~ (∃ n, P n) -> ∀ n, ~ P n.
+  Proof.
+    unfold not; intros notex n abs.
+    apply notex.
+    exists n; trivial.
+  Qed.
+
+  Lemma not_and_imply P Q :
+    ~(P ∧ Q) -> P -> ~Q.
+  Proof. tauto. Qed.
+
+  Lemma not_or_and P Q : ~ (P ∨ Q) -> ~ P ∧ ~ Q.
+  Proof. tauto. Qed.
+
+End ClassicalFacts.
