theories/Commons/WP.v
@@ -1,0 +1,81 @@
+From stdpp Require Import prelude.
+From stdpp Require Import strings.
+
+From RSL Require Import Commons.Language.
+From RSL Require Import Commons.Utils.
+
+(* Set Mangle Names. *)
+
+Section WPProp.
+  Context {Λ: lang} (P: prog Λ).
+
+  Implicit Type s : state Λ.
+
+  Definition final_with Q s : Prop := ∃ v, is_final s = Some v ∧ Q v.
+
+  (** [safe Q n s] : s is a state that is safe for at most n steps:
+      - s is a final step or
+      - s is not stuck and can do at most n steps. *)
+  Inductive safe Q : state Λ -> nat -> Prop :=
+  | safe_init : ∀ s, safe Q s 0
+  | final_is_safe : ∀ s n, final_with Q s -> safe Q s n
+  | safe_to_step : ∀ s n,
+    (* I am not stuck *)
+    can_progress P s ->
+    (* All possible next states are safe for at most n least *)
+    (∀ t, P ⊨ s ->> t -> safe Q t n) ->
+    (* I am safe for at most n+1 least *)
+    safe Q s (S n).
+
+  Lemma safe_from_progress Q s n :
+    (∀ t m, m < n -> P ⊨ s -{m}> t -> final_with Q t ∨ can_progress P t) ->
+    safe Q s n.
+  Proof.
+    induction n as [ | n IH] in s |- *; intros H.
+    - constructor.
+    - assert (Hstep: P ⊨ s -{0}> s) by constructor.
+      assert (Hle: 0 < S n) by lia.
+      destruct (H _ _ Hle Hstep) as [Hfin | Hns]; clear Hstep Hle.
+      + now constructor.
+      + apply safe_to_step; auto. intros t Hstep.
+        apply IH. intros u m Heq Hsteps. subst.
+        apply H with (S m).
+        * lia.
+        * econstructor; now eauto.
+  Qed.
+
+  Lemma safe_implies_progress Q s n :
+    safe Q s n ->
+    ∀ t m, m < n -> P ⊨ s -{m}> t -> final_with Q t ∨ can_progress P t.
+  Proof.
+    intros Hsafe.
+    induction Hsafe as [s' | s' n' Hfin | s' n' Hns Hsafe IH]
+      in n, Hsafe |- *; intros t m Hlt Hrtc.
+    - inv Hlt.
+    - destruct m as [ | m].
+      + inv Hrtc. now left.
+      + exfalso.
+        destruct Hfin as (v & Hfin & HQ). apply nsteps_inv_l in Hrtc.
+        destruct Hrtc as (? & Hstep & ?).
+        eapply mixin_final_no_step; eauto. apply lang_mixin.
+    - destruct m as [ | m ].
+      + inv Hrtc; now auto.
+      + apply nsteps_inv_l in Hrtc.
+        destruct Hrtc as (u & Hstep & Hrtc).
+        eapply IH; try eassumption; lia.
+  Qed.
+
+  Definition safe_mono Q s :
+    ∀ n m, m <= n -> safe Q s n -> safe Q s m.
+  Proof.
+    intros n m Hle Hsafe.
+    induction Hsafe as [ | | ? ? Hns Hsafe IH ] in m, Hle |- *.
+    - inv Hle. constructor.
+    - now apply final_is_safe.
+    - destruct m as [ | m ].
+      + constructor.
+      + apply safe_to_step.
+        * assumption.
+        * intros ? Ht. apply IH; auto. lia.
+  Qed.
+End WPProp.
