theories/RTL/Semantics.v
@@ -1,0 +1,290 @@
+From stdpp Require Import prelude.
+From stdpp Require Import gmap.
+
+From RSL Require Import Commons.Utils.
+From RSL Require Import Commons.Language.
+
+From RSL Require Import RTL.RTL.
+From RSL Require Import RTL.Notations.
+
+Import RTLNotations.
+
+(* Set Mangle Names. *)
+
+Fixpoint init_regs (vl: list val) (rl: list reg) : regmap :=
+  match rl, vl with
+  | r :: rs, v :: vs => <[r := v]>(init_regs vs rs)
+  | _, _ => ∅
+  end.
+
+Inductive stackframe : Type :=
+| Stackframe
+    (res: reg) (* where to store the result *)
+    (f: function) (* calling function *)
+    (pc: node) (* program point in caller function *)
+    (ρ: regmap) (* state in caller function *)
+.
+
+Inductive pcstate : Type :=
+| State
+    (f: function) (* current function *)
+    (pc: node) (* current program point in c *)
+    (ρ: regmap) (* register state *)
+
+| CallState
+    (f: function) (* function to call *)
+    (args: list val) (* arguments to the call *)
+
+| ReturnState
+    (v: val). (* return value for the call *)
+
+Definition rtl_state : Type := list stackframe * pcstate * memory.
+
+Inductive rtl_step (P: program) : rtl_state -> rtl_state -> Prop :=
+| exec_Inop: ∀ σ m ρ f pc pc',
+  f@pc is <{ nop -> pc' }> ->
+  rtl_step P (σ, State f pc ρ, m) (σ, State f pc' ρ, m)
+
+| exec_Iret: forall σ m ρ f pc r v,
+  f@pc is <{ ret r }> ->
+  get_reg r ρ = v ->
+  rtl_step P (σ, State f pc ρ, m) (σ, ReturnState v, m)
+
+| exec_Iop: forall σ m ρ f pc op args dst pc' ρ' v,
+  f@pc is <{ dst := @op args -> pc' }> ->
+  eval_op op (get_regs args ρ) = Some v ->
+  set_reg dst v ρ = ρ' ->
+  rtl_step P (σ, State f pc ρ, m) (σ, State f pc' ρ', m)
+
+| exec_Iload: forall σ m ρ f pc dst src pc' ρ' addr v,
+  f@pc is <{ dst := !src -> pc' }> ->
+  get_reg src ρ = addr ->
+  get_at addr m = Some v ->
+  set_reg dst v ρ = ρ' ->
+  rtl_step P (σ, State f pc ρ, m) (σ, State f pc' ρ', m)
+
+| exec_Istore: forall σ m ρ f pc dst src pc' m' addr v,
+  f@pc is <{ !dst := src -> pc' }> ->
+  get_reg dst ρ = addr ->
+  get_reg src ρ = v ->
+  set_at addr v m = Some m' ->
+  rtl_step P (σ, State f pc ρ, m) (σ, State f pc' ρ, m')
+
+| exec_Icond: forall  σ m ρ f pc cond ifso ifnot v pc',
+  f@pc is <{ if cond then goto ifso else goto ifnot }> ->
+  get_reg cond ρ = v ->
+  pc' = (if Z.eqb v 0 then ifso else ifnot) ->
+  rtl_step P (σ, State f pc ρ, m) (σ, State f pc' ρ, m)
+
+| exec_Icall: forall σ m ρ f pc dst sig args pc' σ' fn,
+  f@pc is <{ dst := @call sig args -> pc' }> ->
+  find_fun P sig = Some fn ->
+  Stackframe dst f pc' ρ :: σ = σ' ->
+  rtl_step P (σ, State f pc ρ, m) (σ', CallState fn (get_regs args ρ), m)
+
+| exec_function: forall σ m ρ f args,
+  length args = length (fn_regs f) ->
+  init_regs args (fn_regs f) = ρ ->
+  rtl_step P (σ, CallState f args, m) (σ, State f (fn_entrypoint f) ρ, m)
+
+| exec_return: forall σ m ρ f pc dst v ρ',
+  set_reg dst v ρ = ρ' ->
+  rtl_step P (Stackframe dst f pc ρ :: σ, ReturnState v, m) (σ, State f pc ρ', m)
+.
+
+Definition is_final (s: rtl_state) : option (val * memory) :=
+  match s with
+  | ([], ReturnState v, m) => Some (v, m)
+  | _ => None
+  end.
+
+Definition can_progress (P: program) s := ∃ t, rtl_step P s t.
+
+
+Lemma rtl_mixin_lang : LangMixin rtl_step can_progress is_final.
+Proof.
+  split.
+  - intros ? [[[] []] ?] ? H [t Hstep]; inv H. inv Hstep.
+  - intros ? [[[] []] ?] ? ? H Hstep; inv H. inv Hstep.
+  - now intros s.
+Qed.
+
+Definition rtl_lang : lang := Lang _ _ _ _ _ _ rtl_mixin_lang.
+
+Section SemProp.
+
+  Let Λ : lang := rtl_lang.
+  Context (P: prog Λ).
+
+  (** Lemmas on the step relation  *)
+  Lemma is_final_struct : ∀ v m s,
+    is_final s = Some (v, m) ->
+    s = ([], ReturnState v, m).
+  Proof. intros v m [[[] []] ?] H; now inv H. Qed.
+
+  Lemma ret_no_nsteps : ∀ n v m s t,
+    is_final s = Some (v, m) ->
+    P ⊨ s -{ n }> t ->
+    t = ([], ReturnState v, m) ∧ n = 0.
+  Proof.
+    intros n v m s t Hfin H.
+    apply is_final_struct in Hfin. subst.
+    destruct n.
+    - now inv H.
+    - destruct (nsteps_inv_l _ _ _ H) as (y & Hstep & _).
+      inv Hstep.
+  Qed.
+
+  Lemma ret_no_step : ∀ v m s t,
+    is_final s = Some (v, m) ->
+    P ⊨ s ->>* t ->
+    t = ([], ReturnState v, m).
+  Proof.
+    intros v m s t Hfin H.
+    destruct (rtc_nsteps_1 _ _ H) as [].
+    eapply ret_no_nsteps; eassumption.
+  Qed.
+
+  (** Lift and Unlift lemmas for step *)
+  Lemma lift_step : ∀ σ σ' Σ s t m m',
+    P ⊨ (σ, s, m) ->> (σ', t, m') ->
+    P ⊨ (σ ++ Σ, s, m) ->> (σ' ++ Σ, t, m').
+  Proof.
+    intros ? ? ? ? ? ? ? H; inv H; econstructor; now eauto.
+  Qed.
+
+  Lemma unlift_step : ∀ σ s m σ' t m' Σ,
+    P ⊨ (σ ++ Σ, s, m) ->> (σ' ++ Σ, t, m') ->
+    P ⊨ (σ, s, m) ->> (σ', t, m').
+  Proof.
+    intros ? ? ? ? ? ? ? H; inv H;
+      rewrite ? app_comm_cons in *;
+      eassert _ by (eapply app_inv_tail; eassumption);
+      subst; econstructor; now eauto.
+  Qed.
+
+  Theorem lift_steps : ∀ σ s m σ' t m' Σ,
+    P ⊨ (σ, s, m) ->>* (σ', t, m') ->
+    P ⊨ (σ ++ Σ, s, m) ->>* (σ' ++ Σ, t, m').
+  Proof.
+    intros σ s m σ' t m' Σ Hrtc.
+    remember (σ, s, m) as x eqn:Hx.
+    remember (σ', t, m') as y eqn:Hy.
+    induction Hrtc as [ y | x y z H Hrtc IH]
+      in σ, s, m, Hx, σ', t, m', Hy |- *.
+    - subst. inv Hy. reflexivity.
+    - subst. destruct y as [[] ?].
+      etransitivity.
+      + apply rtc_once. apply lift_step. eassumption.
+      + eauto.
+  Qed.
+
+  Lemma unfold_call fn : ∀ n res f pc ρ args m σ t m',
+    P ⊨ ([Stackframe res f pc ρ], CallState fn args, m) -{n}> (σ, t, m') ->
+    (∃ σ',
+        σ = σ' ++ [Stackframe res f pc ρ]
+        ∧ P ⊨ ([], CallState fn args, m) -{n}> (σ', t, m'))
+    ∨
+      (∃ m1 m2 v m'',
+          n = 1 + m1 + m2
+          ∧ P ⊨ ([], CallState fn args, m) -{m1}> ([], ReturnState v, m'')
+          ∧ P ⊨ ([], State f pc (set_reg res v ρ), m'') -{m2}> (σ, t, m')
+      ).
+  Proof.
+    intros n.
+    induction n as [ | n IH ];
+      intros res f pc ρ args m σ t m' Hrtc.
+    - inv Hrtc. left. exists []. split; auto. constructor.
+    - apply nsteps_inv_r in Hrtc. destruct Hrtc as ([[] ?] & Hrtc & Hstep).
+      apply IH in Hrtc.
+      destruct Hrtc
+        as [(σ' & -> & Hlift) | (m1 & m2 & v & m'' & Hn & Hcall & Hrest)].
+      + inv Hstep as [ | | | | | | | | ? ? ? ? ? ? v ? ? Hσ];
+          try (left; eexists; split;
+               [ rewrite ? app_comm_cons; reflexivity
+               | eapply nsteps_r; [ now apply Hlift | econstructor; now eauto]
+               ]
+            ).
+        destruct σ'; inv Hσ.
+        * right. exists n, 0, v, m'. repeat split; eauto. constructor.
+        * left. eexists. split.
+          -- reflexivity.
+          -- eapply nsteps_r; [ now apply Hlift | econstructor; now eauto].
+      + inversion Hstep; subst; right; (exists m1, (S m2), v, m''); repeat split;
+          now eauto || (eapply nsteps_r;
+                        [ now apply Hrest | econstructor; now eauto]).
+  Qed.
+
+  Lemma ret_not_stuck : ∀ frame σ v m,
+    can_progress P (frame :: σ, ReturnState v, m).
+  Proof. intros []. repeat econstructor; now eauto. Qed.
+
+  Lemma ret_stuck_in_empty : ∀ v m,
+    ~ can_progress P ([], ReturnState v, m).
+  Proof. intros v m [u H]. inv H. Qed.
+
+  Lemma lift_not_stuck : ∀ σ Σ s m,
+    can_progress P (σ, s, m) ->
+    can_progress P (σ ++ Σ, s, m).
+  Proof. intros σ Σ s m [[[] ?] Ht]. eexists. apply lift_step. eassumption. Qed.
+
+End SemProp.
+
+Section Regs.
+  Lemma get_regs_insert : ∀ regs r v ρ,
+    r ∉ regs ->
+    get_regs regs (<[r := v]> ρ) = get_regs regs ρ.
+  Proof.
+    intros regs r v ρ.
+    induction regs as [|r' regs' IH]; intros Hnotin; [reflexivity |].
+    simpl. f_equal.
+    - unfold get_reg. rewrite (lookup_insert_ne ρ); set_solver.
+    - apply IH. set_solver.
+  Qed.
+
+  Lemma get_regs_init_regs : ∀ regs args,
+    NoDup regs ->
+    length args = length regs ->
+    get_regs regs (init_regs args regs) = args.
+  Proof.
+    intros regs args Hnodup.
+    revert args.
+    induction Hnodup as [|r regs Hnotin Hnodup IH]; intros args Hlen.
+    - destruct args; [reflexivity | discriminate Hlen].
+    - destruct args as [|v args]; [discriminate Hlen |].
+      simpl in Hlen. injection Hlen as Hlen'.
+      simpl. f_equal.
+      + unfold get_reg. now rewrite (lookup_insert_eq (init_regs args regs)).
+      + rewrite get_regs_insert by exact Hnotin.
+        apply IH. exact Hlen'.
+  Qed.
+
+  Lemma get_reg_set_reg_eq : ∀ r v ρ,
+    get_reg r (set_reg r v ρ) = v.
+  Proof.
+    intros r v ρ.
+    unfold get_reg, set_reg.
+    now rewrite (lookup_insert_eq ρ).
+  Qed.
+
+  Lemma get_reg_set_reg_neq : ∀ r r' v ρ,
+    r ≠ r' -> get_reg r (set_reg r' v ρ) = get_reg r ρ.
+  Proof.
+    intros r r' v ρ Hneq.
+    unfold get_reg, set_reg.
+    now rewrite (lookup_insert_ne ρ).
+  Qed.
+End Regs.
+
+Tactic Notation "simpl_reg" "by" tactic3(tac) :=
+  repeat match goal with
+    | _ => progress tac
+    | |- context[get_reg _ (set_reg _ _ _)] =>
+        (rewrite get_reg_set_reg_neq by tac)
+        || (rewrite get_reg_set_reg_eq by tac)
+    | H: get_reg ?r ?rho = _ |- context[get_reg ?r ?rho] =>
+        repeat rewrite H
+    end.
+
+Global Tactic Notation "simpl_reg" :=
+  simpl_reg by repeat (f_equal || lia ||split).
