theories/Refinement/Behaviors.v
@@ -1,0 +1,162 @@
+From stdpp Require Import prelude.
+From Stdlib Require Import Setoid.
+From Coinduction Require Import all.
+
+From RSL.Commons Require Import Utils.
+From RSL.Commons Require Import Language.
+
+(* Set Mangle Names. *)
+
+Section Behavior.
+  Context {Λ: lang} (P: prog Λ).
+  Implicit Type s : state Λ.
+
+  Program Definition diverges_: mon (state Λ -> Prop) :=
+    {| body R s := ∃ s', P ⊨ s ->> s' ∧ R s' |}.
+  Next Obligation. firstorder. Qed.
+
+  Definition diverges : state Λ -> Prop := gfp diverges_.
+
+  Lemma diveges_sound : ∀ f,
+    (∀ n, P ⊨ f n ->> f (S n)) -> diverges (f 0).
+  Proof.
+    intros f Hf. cut (∀ n, diverges (f n)); auto.
+    unfold diverges. coinduction R cih.
+    intros n. exists (f (S n)); auto.
+  Qed.
+
+  Lemma diverges_unroll : ∀ t,
+    diverges t -> ∃ t', P ⊨ t ->> t' ∧ diverges t'.
+  Proof.
+    intros t H. unfold diverges in H. apply (gfp_fp diverges_) in H.
+    inv H. eexists; now eauto.
+  Qed.
+
+  Lemma diverge_iff : ∀ s,
+    (∀ t, P ⊨ s ->>* t -> ∃ u, P ⊨ t ->> u) <->
+    ∀ t, P ⊨ s ->>* t -> diverges t.
+  Proof.
+    intros s. split.
+    - intros Hs. unfold diverges. coinduction R cih.
+      intros t Hrtc. destruct (Hs _ Hrtc) as [u Hstep].
+      exists u. split; auto.
+      apply cih. eapply rtc_r; eassumption.
+    - intros Hdiv t Hrtc. apply Hdiv in Hrtc.
+      destruct (diverges_unroll _ Hrtc) as [u []].
+      now exists u.
+  Qed.
+
+  Variant behavior :=
+  | Terminating (v: value Λ)
+  | Diverging
+  | Unknown.
+
+  (* [beh s] is the set of all the behaviors of [s] *)
+  Inductive beh : behavior -> state Λ -> Prop :=
+  | IsTerminating : ∀ s v,
+      is_final s = Some v ->
+      beh (Terminating v) s
+  | IsDiverging : ∀ s,
+      diverges s ->
+      beh Diverging s
+  | IsStuck : ∀ s,
+      stuck P s ->
+      beh Unknown s
+  | IsSteping : ∀ s t b,
+      beh b t ->
+      P ⊨ s ->> t ->
+      beh b s.
+
+  #[local] Instance beh_elem_state : ElemOf behavior (state Λ) := beh.
+
+  (* [s] is terminating iff there is a execution from [s] to a final state. *)
+  Lemma has_terminating_behavior : ∀ s v,
+    Terminating v ∈ s <-> ∃ t, P ⊨ s ->>* t ∧ is_final t = Some v.
+  Proof.
+    intros s v. split; intros Hbeh.
+    - remember (Terminating v) as b eqn:Hb.
+      induction Hbeh as [ s | | | s t b ? IH Hstep ]; inv Hb; auto.
+      + exists s. now constructor.
+      + destruct (IH eq_refl) as (t' & Hrtc & Hfin). clear IH.
+        exists t'. split; eauto. now apply rtc_l with t.
+    - destruct Hbeh as (t & Hrtc & Hfin).
+      induction Hrtc as [ | s t u Hstep Hrtc IH ].
+      + now constructor.
+      + eapply IsSteping; eauto. now apply IH.
+  Qed.
+
+  (* [s] is diverging iff [s] has a diverging execution *)
+  Lemma has_diverging_behavior : ∀ s,
+    Diverging ∈ s <-> diverges s.
+  Proof.
+    intros s. split; intros Hbeh.
+    - revert s Hbeh. unfold diverges. coinduction R cih.
+      intros s Hbeh. inv Hbeh.
+      + apply (gfp_pfp diverges_) in H.
+        destruct H as (s' & Hstep & Hdiv).
+        exists s'. split; auto. apply cih. apply IsDiverging. assumption.
+      + exists t. split; auto.
+    - now apply IsDiverging.
+  Qed.
+
+  (* [s] has a unknown behavior if [s] reduces to a stuck state. *)
+  Lemma has_stuck_behavior : ∀ s,
+    Unknown ∈ s <-> ∃ t, P ⊨ s ->>* t ∧ stuck P t.
+  Proof.
+    intros s. split; intros Hbeh.
+    - remember Unknown as b eqn:Hb.
+      induction Hbeh as [ | | s | s t b ? IH Hstep ]; inv Hb; auto.
+      + exists s. now split.
+      + destruct (IH eq_refl) as (u & Hrtc & Hstuck).
+        exists u. split.
+        * now apply rtc_l with t.
+        * assumption.
+    - destruct Hbeh as (u & Hrtc & Hstuck).
+      induction Hrtc  as [ | s t u Hstep Hrtc IH].
+      + now constructor.
+      + eapply IsSteping.
+        * now apply IH.
+        * easy.
+  Qed.
+
+  Definition does_end s : Prop :=
+    ∃ t, P ⊨ s ->>* t ∧ ((∃ v, is_final t = Some v) ∨ stuck P t).
+
+  Lemma not_ending_diverges (EM: EM):
+    ∀ s, ~(does_end s) -> ∀ t, P ⊨ s ->>* t -> diverges t.
+  Proof.
+    intros s H. unfold diverges.
+    coinduction R cih.
+    assert (Hs: ∀ t, P ⊨ s ->>* t -> is_final t = None ∧ ~ stuck P t).
+    {
+      intros t Hstep. apply not_ex_all_not with (n := t) in H.
+      pose proof (not_and_imply _ _ H Hstep) as Hnor. clear H Hstep.
+      destruct (not_or_and _ _ Hnor) as [Hnfin Hnstuck]. clear Hnor.
+      split; auto. clear Hnstuck.
+      destruct (is_final t) as [v | ].
+      - exfalso. apply Hnfin. now eexists.
+      - reflexivity.
+    }
+    intros t Hrtc.
+    destruct (Hs t) as [Hnfin Hnstuck]; auto.
+    unfold stuck in Hnstuck.
+    pose proof (DNE EM (can_progress P t)).
+    assert (Hprogress: can_progress P t) by tauto.
+    eapply mixin_can_progress_must_step in Hprogress.
+    - destruct Hprogress as [u Hstep]. exists u. split.
+      + apply Hstep.
+      + apply cih. eapply rtc_r; eassumption.
+    - apply lang_mixin.
+  Qed.
+
+  Theorem every_state_has_beh (EM: EM) : ∀ s, ∃ b, b ∈ s.
+  Proof.
+    intros s. destruct (EM (does_end s)) as [(t & Hrtc & [[v Hfin] | H]) | H].
+    - exists (Terminating v). apply has_terminating_behavior.
+      exists t; auto.
+    - exists Unknown. apply has_stuck_behavior.
+      exists t; auto.
+    - exists Diverging. apply has_diverging_behavior.
+      apply not_ending_diverges with s; auto.
+  Qed.
+End Behavior.
