theories/Refinement/Sim.v
@@ -1,0 +1,58 @@
+From stdpp Require Import prelude.
+From stdpp Require Import tactics.
+
+From Coinduction Require Import all.
+
+From RSL.Commons Require Import Language.
+
+(* Set Mangle Names. *)
+
+Section SimDef.
+  Context {Λₜ Λₛ: lang}.
+  Context (Pₜ: prog Λₜ) (Pₛ: prog Λₛ) (Φ: value Λₜ -> value Λₛ -> Prop).
+
+  Definition is_final (t: state Λₜ) (s: state Λₛ) : Prop :=
+    ∃ vₜ vₛ, is_final t = Some vₜ ∧ is_final s = Some vₛ ∧ Φ vₜ vₛ.
+
+  Inductive sim_lfp'
+    (gfp: state Λₜ -> state Λₛ -> Prop) : state Λₜ -> state Λₛ-> Prop :=
+  | BothFinal : ∀ t s,
+    is_final t s -> sim_lfp' gfp t s
+
+  | SourceStuck : ∀ t s,
+    stuck Pₛ s -> sim_lfp' gfp t s
+
+  | TargetStutter : ∀ t s s',
+    Pₛ ⊨ s ->> s' -> sim_lfp' gfp t s' -> sim_lfp' gfp t s
+
+  | TargetSteps : ∀ t s,
+    can_progress Pₜ t ->
+    (∀ t', Pₜ ⊨ t ->> t' -> sim_lfp' gfp t' s) ->
+    sim_lfp' gfp t s
+
+  | BothSteps : ∀ t s,
+    can_progress Pₜ t ->
+    (∀ t', Pₜ ⊨ t ->> t' -> ∃ s', Pₛ ⊨ s ->> s' ∧ gfp t' s') ->
+    sim_lfp' gfp t s.
+
+  Instance sim_lfp'_proper : Proper (leq ==> leq) sim_lfp'.
+  Proof.
+    intros gfp gfp' Hgfp s t H. induction H as [ | | | | ? ? ? H ];
+      try (econstructor; eassumption || now apply Hlfp).
+    apply BothSteps; eauto. intros t' Hstep.
+    destruct (H _ Hstep) as (? & ? & ?).
+    eexists. split; eassumption || now apply Hgfp.
+  Qed.
+
+  Definition sim_lfp : mon (state Λₜ -> state Λₛ -> Prop) := {| body := sim_lfp' |}.
+
+  Definition sim := gfp sim_lfp.
+
+  Lemma sim_unroll t s :
+    gfp sim_lfp t s -> sim_lfp' (gfp sim_lfp) t s.
+  Proof. apply (gfp_fp sim_lfp). Qed.
+
+  Lemma sim_roll t s :
+    sim_lfp' (gfp sim_lfp) t s -> gfp sim_lfp t s.
+  Proof. apply (gfp_fp sim_lfp). Qed.
+End SimDef.
