theories/Refinement/Sound.v
@@ -1,0 +1,226 @@
+From stdpp Require Import prelude.
+
+From Coinduction Require Import all.
+
+From RSL.Commons Require Import Utils.
+From RSL.Commons Require Import Language.
+
+From RSL.Refinement Require Import Behaviors.
+From RSL.Refinement Require Import Sim.
+
+(* Set Mangle Names. *)
+
+Section SimSound.
+  Context {Λₜ Λₛ: lang}.
+  Context (Pₜ: prog Λₜ) (Pₛ: prog Λₛ).
+
+  Instance behₜ_elem : ElemOf behavior (state Λₜ) := beh Pₜ.
+  Instance behₛ_elem : ElemOf behavior (state Λₛ) := beh Pₛ.
+
+  Inductive behavior_order Φ : @behavior Λₜ -> @behavior Λₛ -> Prop :=
+  | TerminatingOrder : ∀ (vₜ: value Λₜ) (vₛ: value Λₛ),
+    Φ vₜ vₛ -> behavior_order Φ (Terminating vₜ) (Terminating vₛ)
+  | DivergingOrder : behavior_order Φ Diverging Diverging
+  | UnknownOrder : ∀ s, behavior_order Φ s Unknown.
+
+  Notation "a '⊑{' Φ '}' b" :=
+    (behavior_order Φ a b)
+      (at level 70, format "a  '⊑{' Φ '}'  b", no associativity).
+
+  Notation "t '≲' s '{{' Φ '}}'" := (gfp (sim_lfp Pₜ Pₛ Φ) t s).
+
+  Lemma terminating_sim Φ : ∀ t s vₜ,
+    t ≲ s {{ Φ }} ->
+    Terminating vₜ ∈ t ->
+    ∃ b, b ∈ s ∧ Terminating vₜ ⊑{Φ} b.
+  Proof.
+    intros t s vₜ Hsim Hb.
+    (* t Terminates -> it reduces to a final state *)
+    apply has_terminating_behavior in Hb. destruct Hb as (t' & Hrtc & Hfin).
+    revert s Hsim.
+    (* Induction on the reduction *)
+    induction Hrtc as [ t | t u t' Ht Hrtc IHt ]; intros s Hsim.
+    - (* t is final *)
+      apply sim_unroll in Hsim.
+      induction Hsim as [ t s Hfinal
+                        | t s Hstuck
+                        | t s s' Hs _ IHs
+                        | t s Hprogress _
+                        | t s Hprogress _ ].
+      + (* Both Final *)
+        destruct Hfinal as (? & vₛ & Ht & ? & ?).
+        (* s is final too *)
+        inv Ht. exists (Terminating vₛ). now do 2 constructor.
+      + (* Source Stuck *)
+        exists Unknown. split; now constructor.
+      + (* Target Stutter, use IH on s *)
+        destruct (IHs Hfin) as (b & Hbeh & Horder).
+        exists b. split; auto.
+        eapply IsSteping; now eauto.
+      + (* Source Stutter -> contradiction *) mixin.
+      + (* Both Steps -> contradiction *) mixin.
+    - (* t steps *)
+      apply sim_unroll in Hsim.
+      induction Hsim as [ t s Hfinal
+                        | t s Hstuck
+                        | t s s' Hs _ IHs
+                        | t s Hprogress Hsim
+                        | t s Hprogress Hgfp ].
+      + (* Both Final -> contradiction *)
+        destruct Hfinal as (? & ? & ? & ? & ?). mixin.
+      + (* Source Stuck *)
+        exists Unknown. split; now constructor.
+      + (* Target Stutter, use IH on s *)
+        destruct (IHs Ht) as (b & Hbeh & Horder).
+        exists b. split; auto.
+        eapply IsSteping; now eauto.
+      + (* Source Stutter, use IH on t *)
+        apply IHt; auto. apply sim_roll. auto.
+      + (* Both Steps, use IH on t*)
+        destruct (Hgfp _ Ht) as (s' & Hs & Hsim).
+        apply IHt in Hsim; auto.
+        destruct Hsim as (b & Hbeh & ?).
+        exists b. split; auto.
+        eapply IsSteping; eauto.
+  Qed.
+
+  Lemma sim_lfp_progress Φ : ∀ t s,
+    t ≲ s {{ Φ }} ->
+    diverges Pₜ t ->
+    stuck Pₛ s ∨
+      ∃ s', Pₛ ⊨ s ->> s' ∧
+            (
+              (∃ t', t' ≲ s' {{ Φ }} ∧ diverges Pₜ t') ∨
+                (t ≲ s' {{ Φ }} ∧ diverges Pₜ t)
+            ).
+  Proof.
+    intros t s Hsim Hdiv.
+    apply sim_unroll in Hsim.
+    induction Hsim as [ t s Hfin
+                      | t s Hstuck
+                      | t s s' Hstep Hsim' IH
+                      | t s Hprog Hsteps IH
+                      | t s Hprog Hsteps ].
+    - (* BothFinal: Contradiction *)
+      destruct Hfin as (vₜ & vₛ & Ht_fin & Hs_fin & HPhi).
+      apply diverges_unroll in Hdiv. destruct Hdiv as (t' & Ht_step & _).
+      mixin.
+    - (* SourceStuck *)
+      left. exact Hstuck.
+    - (* TargetStutter *)
+      apply sim_roll in Hsim'.
+      right. exists s'. split; now auto.
+    - (* TargetSteps *)
+      (* t can progress, target waits. Because t diverges, it steps to t' *)
+      apply diverges_unroll in Hdiv. destruct Hdiv as (t' & Ht_step & Hdiv_t').
+      (* Apply the IH for t' *)
+      destruct (IH t' Ht_step Hdiv_t') as
+        [Hstuck | (s' & Hstep & [(? & ? & ?) | []])].
+      + now left.
+      + right. eexists. split; eauto.
+      + right. eexists. split; eauto.
+
+    - (* BothSteps *)
+      apply diverges_unroll in Hdiv. destruct Hdiv as (t' & Ht_step & Hdiv_t').
+      destruct (Hsteps t' Ht_step) as (s' & Hs_step & Hsim_next).
+      right. exists s'. split; auto.
+      left. exists t'. split; auto.
+  Qed.
+
+  Lemma diverging_sim (EM: EM) Φ : ∀ t s,
+    t ≲ s {{ Φ }} ->
+    Diverging ∈ t ->
+    ∃ b, b ∈ s ∧ Diverging ⊑{Φ} b.
+  Proof.
+    intros t s Hsim Hdiv.
+    destruct (EM (∃ s', Pₛ ⊨ s ->>* s' ∧ stuck Pₛ s')) as [Hstuck | Hnstuck].
+    - exists Unknown. split; now apply has_stuck_behavior || constructor.
+    - exists Diverging. split; try constructor.
+      apply has_diverging_behavior in Hdiv.
+      assert (H: sim Pₜ Pₛ Φ t s) by exact Hsim. clear Hsim.
+      unfold diverges.
+      revert t s Hdiv H Hnstuck. coinduction R cih.
+      intros t s Hdiv Hsim Hnstuck.
+      destruct (sim_lfp_progress _ _ _ Hsim Hdiv) as
+        [Hstuck | (s' & Hstep & [(t' & ? & ?) | []])].
+      + exfalso. apply Hnstuck. exists s. split; auto.
+      + exists s'. split; auto. apply cih with t'; auto.
+        intros (s'' & ? & ? ).
+        apply Hnstuck. exists s''. split; auto.
+        econstructor; now eauto.
+      + exists s'. split; auto. apply cih with t; auto.
+        intros (s'' & ? & ? ).
+        apply Hnstuck. exists s''. split; auto.
+        econstructor; now eauto.
+  Qed.
+
+  Lemma stuck_sim Φ : ∀ t s,
+    t ≲ s {{ Φ }} ->
+    Unknown ∈ t ->
+    Unknown ∈ s.
+  Proof.
+    intros t s Hsim Hb.
+    (* t reach a stuck state. *)
+    apply has_stuck_behavior in Hb. destruct Hb as (t' & Hrtc & Hstuck).
+    revert s Hsim.
+    (* Induction on the reduction *)
+    induction Hrtc as [ t | t u t' Ht Hrtc IHt ]; intros s Hsim.
+    - (* t = t' *)
+      apply sim_unroll in Hsim.
+      induction Hsim as [ t s Hfinal
+                        | t s ?
+                        | t s s' Hs _ IHs
+                        | t s Hprogress _
+                        | t s Hprogress _ ].
+      + (* Both Final -> contradiction *)
+        destruct Hfinal as (? & vₛ & Ht & ? & ?).
+        mixin.
+      + (* Source Stuck -> trivial *)
+        now constructor.
+      + (* Target Stutter, use IH on s *)
+        eapply IsSteping; eauto.
+        now apply IHs.
+      + (* Source Stutter -> contradiction *) mixin.
+      + (* Both Steps -> contradiction *) mixin.
+    - (* t steps *)
+      apply sim_unroll in Hsim.
+      induction Hsim as [ t s Hfinal
+                        | t s ?
+                        | t s s' Hs _ IHs
+                        | t s Hprogress Hsim
+                        | t s Hprogress Hgfp ].
+      + (* Both Final -> contradiction *)
+        destruct Hfinal as (? & ? & ? & ? & ?). mixin.
+      + (* Source Stuck -> trivial *)
+        now constructor.
+      + (* Target Stutter, use IH on s *)
+        eapply IsSteping; eauto.
+        now apply IHs.
+      + (* Source Stutter, use IH on t *)
+        apply IHt; auto. apply sim_roll. auto.
+      + (* Both Steps, use IH on t *)
+        destruct (Hgfp _ Ht) as (s' & Hs & Hsim).
+        apply IHt in Hsim; auto.
+        eapply IsSteping; now eauto.
+  Qed.
+
+  (* A definition of state refinement: *)
+  (*    - if the target terminates on (v, m), *)
+  (*    the source must either terminate on (v, m) or be stuck. *)
+  (*    - if the target diverges, *)
+  (*    the source must either diverges or be stuck. *)
+  (*    - if the target is stuck, the source should also be stuck. *)
+  Definition refines Φ (t: state Λₜ) (s: state Λₛ) :=
+    ∀ b, b ∈ t -> ∃ b', b' ∈ s ∧ b ⊑{Φ} b'.
+
+  Theorem sim_sound (EM: EM) Φ : ∀ t s,
+    t ≲ s {{ Φ }} -> refines Φ t s.
+  Proof.
+    intros t s Hsim [] Hb.
+    - now apply terminating_sim with t.
+    - now apply diverging_sim with t.
+    - exists Unknown. split.
+      + now apply stuck_sim with (t := t) (Φ := Φ).
+      + now constructor.
+  Qed.
+End SimSound.
